examples/pseudo_bool/cp_encoding/README.md
@@ -1,5 +1,8 @@
 CP semantics and encoders
 
+[array](array):
+CakeML frontends for the CP encoder.
+
 [cpScript.sml](cpScript.sml):
 Definition of CP problem syntax and semantics
 
